Composition/States.v
@@ -2,19 +2,16 @@ From Coq Require Import List Lia RelationClasses.
 From Bythos.Systems Require Export States.
 From Bythos.Composition Require Export Protocol.
 
-Module CompNetState (A : NetAddr) (M1 M2 : MessageType) (BTh : ByzThreshold A)
+Module Type CompNetState (A : NetAddr) (M1 M2 : MessageType) (BTh : ByzThreshold A)
   (CM : CompMessage M1 M2) (Pk1 : SimplePacket A M1) (Pk2 : SimplePacket A M2)
   (CPk : CompSimplePacket A M1 M2 CM Pk1 Pk2)
   (Pt1 : Protocol.Protocol A M1 Pk1 BTh)
   (Pt2 : Protocol.Protocol A M2 Pk2 BTh)
   (SCPT : SeqCompProtocolTrigger A M1 M2 BTh Pk1 Pk2 Pt1 Pt2)
-  (Ns1 : NetState A M1 Pk1 BTh Pt1) (Ns2 : NetState A M2 Pk2 BTh Pt2).
-  (* (CPt : SeqCompProtocol A M1 M2 BTh CM Pk1 Pk2 CPk Pt1 Pt2 SCPT) <: NetState A CM CPk BTh. *)
+  (Ns1 : NetState A M1 Pk1 BTh Pt1) (Ns2 : NetState A M2 Pk2 BTh Pt2)
+  (CPt : SeqCompProtocol A M1 M2 BTh CM Pk1 Pk2 CPk Pt1 Pt2 SCPT) <: NetState A CM CPk BTh CPt.
 
 Import BTh CM CPk SCPT.
-
-(* HMM what if we do Include here ... *)
-Module Export CPt := SeqCompProtocol A M1 M2 BTh CM Pk1 Pk2 CPk Pt1 Pt2 SCPT.
 
 Include NetState A CM CPk BTh CPt.
 
@@ -23,15 +20,17 @@ Definition stmap_proj1 (stmap : StateMap) : Ns1.StateMap := fun n => (stmap n).(
 
 Definition stmap_proj2 (stmap : StateMap) : Ns2.StateMap := fun n => (stmap n).(st2).
 
-Definition world_proj1 (w : SystemState) : Ns1.SystemState :=
+Definition sysstate_proj1 (w : SystemState) : Ns1.SystemState :=
   Ns1.mkW (stmap_proj1 (localState w)) (pkts_filter_proj1 (packetSoup w)).
 
-Definition world_proj2 (w : SystemState) : Ns2.SystemState :=
+Definition sysstate_proj2 (w : SystemState) : Ns2.SystemState :=
   Ns2.mkW (stmap_proj2 (localState w)) (pkts_filter_proj2 (packetSoup w)).
 
 Local Set Implicit Arguments.
 
-Fact procMsgWithCheck_proj1 [st src m1] : forall st' pkts,
+(* very trivial lemmas *)
+
+Fact procMsg_proj1 [st src m1] : forall st' pkts,
   procMsg st src (inl m1) = (st', pkts) ->
   let: res := Pt1.procMsg st.(st1) src m1 in
   st'.(st1) = fst res /\ pkts_filter_proj1 pkts = snd res.
@@ -57,7 +56,7 @@ Proof.
   all: simpl; now autorewrite with pkts_filter.
 Qed.
 
-Fact procMsgWithCheck_proj2 [st src m2] : forall st' pkts,
+Fact procMsg_proj2 [st src m2] : forall st' pkts,
   procMsg st src (inr m2) = (st', pkts) ->
   let: res := Pt2.procMsg st.(st2) src m2 in
   st'.(st2) = fst res /\ pkts_filter_proj2 pkts = snd res.
