Protocols/RBABC/Types.v
@@ -1,7 +1,6 @@
 From Coq Require Import List.
 From Coq Require ssrbool.
 Import (coercions) ssrbool.
-From Bythos.Composition Require Export Types.
 From Bythos.Protocols.ABC Require Export Types.
 From Bythos.Protocols.RB Require Export Types.
 
@@ -9,19 +8,11 @@ From Bythos.Protocols.RB Require Export Types.
     then it is possible for adversaries to collect signatures from different instances
     and use them in one particular instance.
   in this case, we need to change the protocol a little bit ...
+  choose either:
   (1) we only allow one instance of ABC for some (node, round) pair. 
   (2) the value of ABC to be signed becomes the product of instance id and value. 
 *)
-(*
-Module Export SingleRound <: Round.
 
-Definition Round := unit.
-Definition Round_eqdec : forall r1 r2 : Round, {r1 = r2} + {r1 <> r2}.
-  intros [][]. left. reflexivity.
-Qed.
-
-End SingleRound.
-*)
 Module Type AddrRoundPair (Export A : NetAddr) (Export R : Round).
 
 Parameter arp : Address * Round.
